proof/Poly/Base.v
@@ -3,7 +3,6 @@ Require Export BaseNat.
 Require Export BaseTactics.
 Require Import Coq.Arith.Compare.
 
-
 (* Cases library due to Aaron Bohannon ********************)
 Require String. Open Scope string_scope.
 
